MyMain.thy
@@ -44,18 +44,16 @@ lemma "eval (MyOCL.As self MyOCL.LECTURERS) (OM ps es)
    apply auto
   done
 
-(* self.lecturers\<rightarrow>size() \<equiv> SELECT COUNT(lecturers) FROM Enrollment WHERE students = self *)
-lemma "eval (MyOCL.Size (MyOCL.As self MyOCL.LECTURERS)) (OM ps es)
-= exec (SelectFromWhere (MySQL.Count MySQL.LECTURERS) 
-(Table ENROLLMENT)
-(WHERE (MySQL.Eq (MySQL.Col (MySQL.STUDENTS)) (MySQL.Var self)))) (OM ps es)"
-  apply auto
-  apply(simp add: lem4)
-  apply (induct es)
-   apply auto
-  sorry 
-
 lemma opp_opp: "opposite (opposite col) = col"
+  sorry
+
+lemma ass1 : "filterWhere (TEnrollment (OM ps [])) (WHERE exp) = (VList [])"
+  sorry
+
+lemma ass2 : "filterWhere (TEnrollment (OM ps (v#vs))) (WHERE exp) = (
+if (isTrue (VList (select (VEnrollment v) exp)))  
+    then (appendList (VEnrollment v) (filterWhere (VList (mapEnrollmentToValList vs)) (WHERE exp)))   
+    else filterWhere (VList (mapEnrollmentToValList vs)) (WHERE exp))"
   sorry
 
 lemma EqualSize_extEnrollment_extCol : "sizeVal (VList (extEnrollment var col enrollments)) 
@@ -64,6 +62,19 @@ lemma EqualSize_extEnrollment_extCol : "sizeVal (VList (extEnrollment var col en
    apply(simp)
   apply(simp add: opp_opp)
   done
+
+
+(* self.lecturers\<rightarrow>size() \<equiv> SELECT COUNT *  FROM Enrollment WHERE students = self *)
+lemma "eval (MyOCL.Size (MyOCL.As self MyOCL.LECTURERS)) (OM ps es)
+= exec (SelectFromWhere (MySQL.Count MySQL.LECTURERS) 
+(Table ENROLLMENT)
+(WHERE (MySQL.Eq (MySQL.Col (MySQL.STUDENTS)) (MySQL.Var self)))) (OM ps es)"
+  apply auto
+  apply(simp_all add: lem4)
+  apply (induct es)
+   apply auto
+  done 
+
 
 (* self.lecturers\<rightarrow>isEmpty() \<equiv> SELECT COUNT * = 0 FROM Enrollment WHERE students = self *)
 lemma "eval (MyOCL.IsEmpty (MyOCL.As self MyOCL.LECTURERS)) (OM ps es)
@@ -76,15 +87,25 @@ lemma "eval (MyOCL.IsEmpty (MyOCL.As self MyOCL.LECTURERS)) (OM ps es)
   apply auto
   done  
 
+lemma sizeVal_appendList : "sizeVal (appendList (VString s) vs) = Suc (sizeVal vs)"
+  apply(induct vs)
+  apply(simp_all)
+  sorry
+
 (* self.lecturers\<rightarrow>exists(l|l=caller)  = SELECT COUNT *  > 0 FROM Enrollment WHERE self = students
 AND lecturers = caller *)
 lemma "eval (MyOCL.Exists (MyOCL.As self MyOCL.LECTURERS) (l) 
-(MyOCL.Eq (MyOCL.Var l) (MyOCL.Var caller))) om
+(MyOCL.Eq (MyOCL.Var l) (MyOCL.Var caller))) (OM ps es)
 =
 exec ((SelectFromWhere (MySQL.GrtThan (CountAll) (MySQL.Int 0)) (Table ENROLLMENT) 
 (WHERE (MySQL.And (MySQL.Eq (MySQL.Var self) (Col col.STUDENTS)) 
-(MySQL.Eq (MySQL.Var caller) (Col col.LECTURERS)))))) om"
+(MySQL.Eq (MySQL.Var caller) (Col col.LECTURERS)))))) (OM ps es)"
   apply auto
+  apply (induct es)
+   apply(simp add:ass1)
+  apply auto
+  apply (simp add: sizeVal_appendList ass2)
+
 
 end
 
